place graph is type ntree, maybe change to list ntree

execution/theories/ContractSystems.v
@@ -4,11 +4,14 @@ From Coq Require Import List.
 From Coq Require Import String.
 From Coq Require Import Sets.Ensembles.
 From Coq Require Import ZArith.
+From Coq Require Import ProofIrrelevance.
 From ConCert.Execution Require Import ChainedList.
 From ConCert.Execution Require Import Blockchain.
 From ConCert.Execution Require Import Serializable.
 From ConCert.Execution Require Import ResultMonad.
 From ConCert.Execution Require Import ContractMorphisms.
+
+Import ListNotations.
 
 Axiom todo : forall {A}, A.
 
@@ -17,105 +20,395 @@ Axiom todo : forall {A}, A.
 Section ContractSystem.
 Context {Base : ChainBase}.
 
-(** Contract systems are organized via some inductive constructor, e.g. lists, trees, or forests *)
-Class Sys_Constr (sys_constr : Type -> Type) := { 
-    (* some utilities for sys_constr : find, update, in predicate, and accum *)
-    places : Type ; (* to traverse constr T for any T, e.g. nat for constr = list *)
-    constr_find : forall {T} (place : places) (struct : sys_constr T), option T ;
-    update : forall {T} (place : places) (t : T) (struct : sys_constr T), sys_constr T ;
-    in_constr : forall {T} (t : T) (struct : sys_constr T), Prop ;
-    sys_accum : forall {T}, sys_constr T -> option T ; (* accumulates into a single value of T *)
-    (* sys_constr has inner and outer merge semantics *)
-    inner_names : forall {T}, sys_constr T -> Type ;
-    outer_names : forall {T}, sys_constr T -> Type ;
-    inner_merge : forall {T} (sys1 : sys_constr T), sys_constr T -> inner_names sys1 -> sys_constr T ;
-    outer_merge : forall {T} (sys1 : sys_constr T), sys_constr T -> outer_names sys1 -> sys_constr T ;
-    (* sys_constr has an automorphism group *)
-    constr_permutation : forall {T}, sys_constr T -> sys_constr T -> Prop ;
-    constr_permutation_in : forall {T} (t : T) struct struct', 
-        constr_permutation struct struct' ->
-        in_constr t struct -> in_constr t struct' ;
-    (* functions between systems : sys_constr is functorial wrt most of ^^ *)
-    constr_funct : forall {T T'}, (T -> T') -> (sys_constr T -> sys_constr T') ;
-    constr_funct_A : forall {T T'}, (T -> T') -> (places -> places) ;
-    constr_find_funct : forall {T T'} (f : T -> T') place struct,
-        constr_find (constr_funct_A f place) (constr_funct f struct) = 
-        option_map f (constr_find place struct) ;
-    update_funct : forall {T T'} (f : T -> T') place t struct, 
-        update (constr_funct_A f place) (f t) (constr_funct f struct) = 
-        constr_funct f (update place t struct) ;
-    in_constr_funct : forall {T T'} (f : T -> T') t struct,
-        in_constr t struct -> in_constr (f t) (constr_funct f struct) ;
-    (* TODO possibly add merge functoriality here too *)
+(** The fundamental building block of a system: a contract and its address *)
+Record GeneralizedContract := {
+    gc_addr : Address ; (* an affiliated address *)
+    gc_wc : WeakContract ; (* wc representation, to deal with polymorphism *)
 }.
 
-(* assume some system construction sys_constr *)
-Context `{Sys_Constr sys_constr}.
+(** The definition of a contract's Place Graph *)
+Section PlaceGraph.
+
+(* an inductive definition of trees *)
+Section NTree.
+
+Inductive ntree (T : Type) : Type :=
+| Leaf : ntree T
+| Node : T -> list (ntree T) -> ntree T.
+
+(** Utils *)
+Fixpoint replace_at_index {T : Type} (n : nat) (new_elem : T) (l : list T) : list T :=
+  match l, n with
+  | nil, _ => nil
+  | _ :: tl, 0 => new_elem :: tl
+  | hd :: tl, S n' => hd :: replace_at_index n' new_elem tl
+  end.
+
+(* Update a tree at a given index, which can be at a node or a leaf *)
+Fixpoint update_ntree_at_index {T : Type} (tree : ntree T) (value : T) (leaf_index : list nat) : ntree T :=
+  match tree, leaf_index with
+  | Leaf _, nil => Node T value nil
+  | Leaf _, _ :: _ => tree (* Cannot add a node at a leaf that does not exist *)
+  | Node _ v children, nil => Node T value children (* Reached the desired leaf *)
+  | Node _ v children, i :: is =>
+      match List.nth_error children i with
+      | Some child => Node T v (replace_at_index i (update_ntree_at_index child value is) children)
+      | None => tree (* Invalid leaf index *)
+      end
+  end.
+
+(* Merge semantics: add a tree to a given leaf *)
+Fixpoint add_tree_at_leaf {T} (orig append : ntree T) (leaf_index : list nat) : ntree T :=
+    match orig, leaf_index with
+    | Leaf _, nil => append
+    | Leaf _, _ :: _ => orig (* Cannot add a tree at a leaf that does not exist *)
+    | Node _ v children, nil => orig (* Must add only at a leaf *)
+    | Node _ v children, i :: is =>
+        match List.nth_error children i with
+        | Some child => Node T v (replace_at_index i (add_tree_at_leaf child append is) children)
+        | None => orig (* Invalid leaf index *)
+        end
+    end.
+
+(* find the leaves of a tree *)
+Definition find_leaf_indices {T : Type} (tree : ntree T) (prefix : list nat) : list (list nat) := todo. (*
+Fixpoint find_leaf_indices {T : Type} (tree : ntree T) (prefix : list nat) : list (list nat) := todo.
+    match tree with 
+    | Leaf _ => t (* we've reached a leaf *)
+    | Node _ v children => 
+        List.fold_left 
+        (fun (prefix' : list (list nat)) (child : ntree T) : list (list nat) => 
+            List.fold_left
+            (fun (l1 l2 : list (list nat)) => l1 ++ l2)
+            (find_leaf_indices child prefix)
+            [])
+        children
+        prefix
+    end.
+*)
+
+Fixpoint ntree_find_node {T} (leaf_index : list nat) (tree : ntree T) : option T :=
+    match tree, leaf_index with 
+    | Leaf _, nil => None (* The index was for a leaf *)
+    | Leaf _, _ :: _ => None (* Cannot find a node that does not exist *)
+    | Node _ v children, nil => Some v (* Reached the desired node *)
+    | Node _ v children, i :: is =>
+        match List.nth_error children i with
+        | Some child => ntree_find_node is child (* Iterate *)
+        | None => None (* Invalid leaf index *)
+        end
+    end.
+
+Definition empty_ntree {T} := Leaf T.
+
+Definition singleton_ntree {T} (t : T) := Node T t nil.
+
+Definition in_ntree {T} (t : T) (tree : ntree T) : Prop := 
+    exists leaf_index, ntree_find_node leaf_index tree = Some t.
+
+(* Given an accumulating function and a starting point, iterate over the tree *)
+Fixpoint ntree_accum {T} (tree : ntree T) (accum : T -> T -> T) (t : T) : T :=
+    match tree with 
+    | Leaf _ => t (* we've reached a leaf *)
+    | Node _ v children => 
+        List.fold_left 
+        (fun (t' : T) (child : ntree T) => accum (ntree_accum child accum t) t')
+        children
+        (accum v t)
+    end.
+(*
+Compute (ntree_accum 
+    (Node nat 1 [singleton_ntree 2 ; singleton_ntree 4 ; singleton_ntree 5])
+    (fun (a b : nat) => a + b)
+    0).
+
+Compute 
+    find_leaf_indices
+    (Node nat 1 [singleton_ntree 2 ; singleton_ntree 4 ; singleton_ntree 5])
+    [1;2;3].
+*)
 
 
-(** We define a system of contracts *)
+(** Functoriality *)
+Fixpoint ntree_funct {T T'} (f : T -> T') (tree : ntree T) : ntree T' := 
+    match tree with 
+    | Leaf _ => Leaf T' 
+    | Node _ v children => 
+        Node T' (f v) (List.map (fun child => ntree_funct f child) children)
+    end.
+
+Lemma ntree_find_funct {T T'} (f : T -> T') (index : list nat) (tree : ntree T) : 
+    ntree_find_node index (ntree_funct f tree) = 
+    option_map f (ntree_find_node index tree).
+Proof.
+    unfold ntree_find_node, ntree_funct.
+    cbn.
+    destruct tree, index; auto.
+Admitted.
+
+Lemma ntree_update_funct {T T'} (f : T -> T') index t tree : 
+    update_ntree_at_index (ntree_funct f tree) (f t) index = 
+    ntree_funct f (update_ntree_at_index tree t index).
+Admitted.
+
+Lemma in_ntree_funct {T T'} (f : T -> T') t tree :
+    in_ntree t tree -> in_ntree (f t) (ntree_funct f tree).
+Proof.
+    intro in_tree.
+    destruct in_tree as [index is_in].
+    unfold in_ntree.
+    exists index.
+    rewrite ntree_find_funct.
+    now rewrite is_in.
+Qed.
+
+
+(** Permutations *)
+Definition NTree_Permutation {T} : ntree T -> ntree T -> Prop := todo.
+
+Lemma intree_permutation_in {T} t (ntree1 ntree2 : ntree T) : 
+    NTree_Permutation ntree1 ntree2 -> 
+    (in_ntree t ntree1 <-> in_ntree t ntree2).
+Proof.
+    intro premute.
+    split.
+    (* -> *)
+    -   admit.
+    (* <- *)
+    -   admit.
+Admitted.
+
+End NTree.
+
+End PlaceGraph.
+
+
+(** Edges in the link graph are given by contract calls *)
+Section LinkGraph.
+
+(* the system's graph *)
+Definition call_to call : option Address := 
+    match call with 
+    | act_transfer _ _ => None 
+    | act_call addr _ _ => Some addr 
+    | act_deploy _ _ _ => None 
+    end.
+
+(* The type of edges *)
+Record LinkGraphEdges (G1 G2 : GeneralizedContract) : Type := {
+    e_chain : Chain ; 
+    e_ctx : ContractCallContext ; 
+    e_prvstate : SerializedValue ; (* prev state *)
+    e_msg : option SerializedValue ; (* msg *)
+    e_newstate : SerializedValue ; (* new state *)
+    e_nacts : list ActionBody ;
+    linking_act : ActionBody ; (* the action that links the two contracts *)
+    (* there is some transaction for which G1 calls G2 *)
+    e_recv_some : 
+        (* this is a successful call *)
+        wc_receive (gc_wc G1) e_chain e_ctx e_prvstate e_msg = Ok (e_newstate, e_nacts) /\
+        (* which emits the transaction linking_act, *)
+        List.In linking_act e_nacts /\ 
+        (* and it is a call to G2 *)
+        call_to linking_act = Some (gc_addr G2) ;
+}.
+
+(* edges can be composed if they are sequential transactions *)
+Definition edges_compose G1 G2 G3 (e1 : LinkGraphEdges G1 G2) (e2 : LinkGraphEdges G2 G3) := 
+    match linking_act G1 G2 e1 with 
+    | act_call _ _ msg => e_msg G2 G3 e2 = Some msg
+    | _ => False
+    end.
+
+End LinkGraph.
+
+
+(** A system of contracts is a (list of) place graphs, 
+    endowed automatically with the link graph structure *)
 Section SystemDefinition.
 
-Record GeneralizedContract := {
-    addr : Address ; (* an affiliated address *)
-    wc : WeakContract ; (* wc representation, to deal with polymorphism *)
-}.
+(* A system of contracts is presented by its place graph;
+    it inherits the link graph automatically *)
+Definition ContractSystem := ntree GeneralizedContract.
 
-Definition ContractSystem := sys_constr GeneralizedContract.
-
-Definition sys_deployed bstate (sys : ContractSystem) : Prop :=
-    forall G,
-    in_constr G sys ->
-    env_contracts bstate (addr G) = Some (wc G).
-
-(** System state  *)
-Definition GeneralizedState : Type := sys_constr (option SerializedValue).
+(** System state *)
+Definition GeneralizedState : Type := ntree (option SerializedValue).
 
 (* the system state is constructed with the same inductive structure as the system *)
 Definition sys_state (bstate : ChainState) (sys : ContractSystem) : GeneralizedState := 
-    constr_funct
-    (fun (gc : GeneralizedContract) => env_contract_states bstate (addr gc))
+    ntree_funct
+    (fun (gc : GeneralizedContract) => env_contract_states bstate (gc_addr gc))
     sys.
 
-(* use sys_accum to compress the state into a single value *)
+(* use sys_accum to compress the state into a single value *) (* TODO remove "serialize tt" somehow 
 Definition sys_state_compressed (bstate : ChainState) (sys : ContractSystem) : option SerializedValue :=
-    match sys_accum (sys_state bstate sys) with 
-    | Some sys_accum => sys_accum 
-    | None => None 
-    end.
+    ntree_accum
+    (sys_state bstate sys)
+    (fun s1 s2 => 
+        match s1, s2 with 
+        | Some x1, Some x2 => Some (serialize (x1, x2))
+        | None, _ => s2 
+        | _, None => s1
+        end)
+    (Some (serialize tt)).
+*)
 
 (** System interface *)
 Record GeneralizedMsg := {
     msg : option SerializedValue ;
-    place : places ; (* the index of *which* contract gets called *)
+    place : list nat ; (* the index of *which* contract gets called *)
 }.
 
 (* move from Generalized State to Generalized State *)
-Definition gen_receive (sys : ContractSystem)
+Definition sys_receive (sys : ContractSystem)
     (c : Chain)
     (ctx : ContractCallContext)
     (g_st : GeneralizedState) (* state *)
     (g_msg : GeneralizedMsg) (* message *) :
     result (GeneralizedState * list ActionBody) SerializedValue := 
-    match constr_find (place g_msg) sys with 
+    match ntree_find_node (place g_msg) sys with 
     | Some gc => 
-        match constr_find (place g_msg) g_st with 
+        match ntree_find_node (place g_msg) g_st with 
         | Some st_op => 
             match st_op with 
             | Some st => 
-                match wc_receive (wc gc) c ctx st (msg g_msg) with 
+                match wc_receive (gc_wc gc) c ctx st (msg g_msg) with 
                 | Ok (new_st, new_acts) => 
-                    Ok (update (place g_msg) (Some new_st) g_st, new_acts)
+                    Ok (update_ntree_at_index g_st (Some new_st) (place g_msg), new_acts)
                 | Err e => Err e
                 end
             | None => Err (serialize tt)
             end
-        | None => Err (serialize tt) (* todo .. is this ok? *)
+        | None => Err (serialize tt)
         end
-    | None => Err (serialize tt) (* todo .. is this ok? *)
+    | None => Err (serialize tt)
     end.
 
 End SystemDefinition.
+
+
+(** Contract System Utils *)
+Section SystemUtils.
+
+(* a system is deployed *)
+Definition sys_deployed bstate (sys : ContractSystem) : Prop :=
+    forall G,
+    in_ntree G sys ->
+    env_contracts bstate (gc_addr G) = Some (gc_wc G).
+
+(* the notion of the initial state of a system *)
+Definition is_genesis_state_wc W init_cstate : Prop := 
+    exists init_chain init_ctx init_setup, 
+    wc_init W init_chain init_ctx init_setup = Ok init_cstate.
+
+(* a better version of this perhaps? *)
+Definition is_genesis_gstate_sys sys gstate : Prop :=
+    forall place,
+    ((exists G, ntree_find_node place sys = Some G) <->
+     (exists st, ntree_find_node place gstate = Some (Some st))) /\
+    (forall place G st, 
+        ntree_find_node place sys = Some G ->
+        ntree_find_node place gstate = Some (Some st) ->
+        is_genesis_state_wc (gc_wc G) st).    
+
+(* some propositions relating to system morphisms *)
+Definition sys_genesis_prop sys1 sys2 
+    (gstate_morph : GeneralizedState -> GeneralizedState) : Prop :=
+    forall gstate,
+        is_genesis_gstate_sys sys1 gstate -> 
+        is_genesis_gstate_sys sys2 (gstate_morph gstate).
+
+Definition sys_coherence_prop sys1 sys2 
+    (gstate_morph : GeneralizedState -> GeneralizedState)
+    (gmsg_morph : GeneralizedMsg -> GeneralizedMsg)
+    (gerror_morph : SerializedValue -> SerializedValue) : Prop := 
+    forall c ctx gst gmsg,
+        result_functor (fun '(gst, l) => (gstate_morph gst, l)) gerror_morph
+            (sys_receive sys1 c ctx gst gmsg) = 
+        sys_receive sys2 c ctx (gstate_morph gst) (gmsg_morph gmsg).
+
+End SystemUtils.
+
+
+Section SystemMorphism.
+
+(* a morphism of systems of contracts *)
+Record SystemMorphism sys1 sys2 := 
+    build_sys_morphism {
+        (* component morphisms *)
+        gstate_morph : GeneralizedState -> GeneralizedState ;
+        gmsg_morph : GeneralizedMsg -> GeneralizedMsg ;
+        gerror_morph : SerializedValue -> SerializedValue ;
+        (* init coherence analogue *)
+        sys_genesis : forall gstate,
+            is_genesis_gstate_sys sys1 gstate ->
+            is_genesis_gstate_sys sys2 (gstate_morph gstate) ;
+        (* recv coherence analogue *)
+        sys_coherence : forall c ctx gst gmsg,
+            result_functor (fun '(gst, l) => (gstate_morph gst, l)) gerror_morph
+                (sys_receive sys1 c ctx gst gmsg) =
+            sys_receive sys2 c ctx (gstate_morph gst) (gmsg_morph gmsg) ;
+}.
+
+Proposition eq_sm {sys1 sys2} (f g : SystemMorphism sys1 sys2) :
+    gstate_morph sys1 sys2 f = gstate_morph sys1 sys2 g -> 
+    gmsg_morph sys1 sys2 f = gmsg_morph sys1 sys2 g -> 
+    gerror_morph sys1 sys2 f = gerror_morph sys1 sys2 g -> 
+    f = g.
+Proof.
+    intros gst_eq gmsg_eq gerr_eq.
+    destruct f, g.
+    simpl in *.
+    subst.
+    f_equal; apply proof_irrelevance.
+Qed.
+
+Definition compose_sm {sys1 sys2 sys3} 
+    (g : SystemMorphism sys2 sys3) (f : SystemMorphism sys1 sys2) : SystemMorphism sys1 sys3.
+Proof.
+    destruct g, f.
+    apply (build_sys_morphism sys1 sys3 
+        (compose gstate_morph0 gstate_morph1)
+        (compose gmsg_morph0 gmsg_morph1)
+        (compose gerror_morph0 gerror_morph1)).
+    -   intros * is_gen.
+        now apply sys_genesis0, sys_genesis1.
+    -   intros.
+        cbn.
+        rewrite <- (sys_coherence0 c ctx (gstate_morph1 gst) (gmsg_morph1 gmsg)).
+        rewrite <- (sys_coherence1 c ctx gst gmsg).
+        unfold result_functor.
+        now destruct (sys_receive sys1 c ctx gst gmsg).
+Defined.
+
+Proposition compose_sm_assoc {sys1 sys2 sys3 sys4}
+    (f : SystemMorphism sys1 sys2)
+    (g : SystemMorphism sys2 sys3)
+    (h : SystemMorphism sys3 sys4) : 
+    compose_sm h (compose_sm g f) = 
+    compose_sm (compose_sm h g) f.
+Proof.
+    now apply eq_sm; unfold compose_sm; destruct f, g, h; cbn.
+Qed.
+
+Definition id_sm sys : SystemMorphism sys sys.
+Proof.
+    apply (build_sys_morphism sys sys id id id); auto.
+    intros.
+    unfold result_functor.
+    simpl.
+    now destruct (sys_receive sys c ctx gst gmsg).
+Qed.
+
+Definition is_iso_sm {sys1 sys2} (f : SystemMorphism sys1 sys2) (g : SystemMorphism sys2 sys1) :=
+    compose_sm g f = id_sm sys1 /\
+    compose_sm f g = id_sm sys2.
+
+Definition sys_isomorphic sys1 sys2 : Prop := 
+    exists (f : SystemMorphism sys1 sys2) (g : SystemMorphism sys2 sys1),
+    is_iso_sm f g.
+
+End SystemMorphism.
 
 
 (** We define various ways in which systems of contracts can be considered equivalent *)
@@ -123,14 +416,14 @@ Section ContractSystemEquivalence.
 
 (** Firstly, a permutation is a strong notion of equality -- they are essentially "identical" *)
 Definition sys_eq (sys1 sys2 : ContractSystem) : Prop := 
-    constr_permutation sys1 sys2.
+    NTree_Permutation sys1 sys2.
 
-(** Secondly, systems are isomorphic if they are isomorphic at every place *)
-Section Isomorphic.
+(** Secondly, systems are isomorphic iff they are isomorphic at every place *)
+Section PlaceIsomorphic.
 
 Record gc_iso (G1 G2 : GeneralizedContract) := {
-    gc_addr_iso : addr G1 = addr G2 ;
-    gc_wc_iso : wc_isomorphic (wc G1) (wc G2) ;
+    gc_addr_iso : gc_addr G1 = gc_addr G2 ;
+    gc_wc_iso : wc_isomorphic (gc_wc G1) (gc_wc G2) ;
 }.
 
 Definition gc_iso_op (g1 g2 : option GeneralizedContract) : Prop := 
@@ -148,11 +441,17 @@ Definition gc_iso_op (g1 g2 : option GeneralizedContract) : Prop :=
     end.
 
 (* the contracts of sys1 and sys2 are isomorphic at every place *)
-Definition sys_isomorphic (sys1 sys2 : ContractSystem) : Prop := 
+Definition sys_place_isomorphic (sys1 sys2 : ContractSystem) : Prop := 
     forall place,
-    gc_iso_op (constr_find place sys1) (constr_find place sys2).
+    gc_iso_op (ntree_find_node place sys1) (ntree_find_node place sys2).
 
-End Isomorphic.
+(* CONJECTURE *)
+Proposition place_iso_equiv : forall sys1 sys2,
+    sys_place_isomorphic sys1 sys2 <->
+    sys_isomorphic sys1 sys2.
+Admitted.
+
+End PlaceIsomorphic.
 
 
 (** Thirdly, systems of contracts can be equivalent by bisimulation *)
@@ -160,18 +459,20 @@ Section Bisimulation.
 
 (** The notion of a system's trace *)
 Section SystemTrace.
-Record SystemStep (sys : ContractSystem) (st1 st2 : GeneralizedState) := {
+Record SystemStep (sys : ContractSystem) (st1 st2 : GeneralizedState) := 
+    build_system_step {
     sys_chain : Chain ; 
     sys_ctx : ContractCallContext ; 
-    sys_gst : GeneralizedState ;
     sys_gmsg : GeneralizedMsg ; 
     sys_new_acts : list ActionBody ;
     (* receive is called successfully *)
-    sys_recv_some : gen_receive sys sys_chain sys_ctx sys_gst sys_gmsg = Ok (st2, sys_new_acts) ;
+    sys_recv_some : sys_receive sys sys_chain sys_ctx st1 sys_gmsg = Ok (st2, sys_new_acts) ;
 }.
 
 Definition SystemTrace (sys : ContractSystem) :=
     ChainedList GeneralizedState (SystemStep sys).
+
+End SystemTrace.
 
 (** Morphism of system traces *)
 Record SystemTraceMorphism (sys1 sys2 : ContractSystem) := 
@@ -179,8 +480,11 @@ Record SystemTraceMorphism (sys1 sys2 : ContractSystem) :=
         (* state morphs, parameterized by states *)
         st_gstate_morph : GeneralizedState -> GeneralizedState ;
         (* some sort of init morph? *)
+        st_genesis_fixpoint : forall (init_gstate : GeneralizedState),
+            is_genesis_gstate_sys sys1 init_gstate ->
+            is_genesis_gstate_sys sys2 (st_gstate_morph init_gstate) ;
         (* step *)
-        sysstep_morph : forall gstate1 gstate2,
+        sys_step_morph : forall gstate1 gstate2,
             SystemStep sys1 gstate1 gstate2 -> 
             SystemStep sys2 (st_gstate_morph gstate1) (st_gstate_morph gstate2) ;
     }.
@@ -194,33 +498,79 @@ Definition compose_stm {sys1 sys2 sys3 : ContractSystem}
     (m2 : SystemTraceMorphism sys2 sys3) (m1 : SystemTraceMorphism sys1 sys2) : 
     SystemTraceMorphism sys1 sys3.
 Proof.
-    apply (build_st_morph sys1 sys3 (compose (st_gstate_morph sys2 sys3 m2) (st_gstate_morph sys1 sys2 m1))).
-    intros.
-    apply (sysstep_morph sys2 sys3 m2).
-    now apply (sysstep_morph sys1 sys2 m1).
-Qed.
+    apply (build_st_morph sys1 sys3 
+        (compose (st_gstate_morph sys2 sys3 m2) (st_gstate_morph sys1 sys2 m1))).
+    -   intros * gen_state1.
+        apply (st_genesis_fixpoint sys2 sys3 m2).
+        now apply (st_genesis_fixpoint sys1 sys2 m1).
+    -   intros * sys_step.
+        apply (sys_step_morph sys2 sys3 m2).
+        now apply (sys_step_morph sys1 sys2 m1).
+Defined.
 
+(* a strong bisimulation *)
 Definition is_iso_stm {sys1 sys2 : ContractSystem}
     (m1 : SystemTraceMorphism sys1 sys2) (m2 : SystemTraceMorphism sys2 sys1) :=
     compose_stm m2 m1 = id_stm sys1 /\ 
     compose_stm m1 m2 = id_stm sys2.
 
-End SystemTrace.
+Definition sm_lift_stm {sys1 sys2} 
+    (f : SystemMorphism sys1 sys2) : SystemTraceMorphism sys1 sys2.
+Proof.
+    apply (build_st_morph sys1 sys2 (gstate_morph sys1 sys2 f) (sys_genesis sys1 sys2 f)).
+    intros * s_step.
+    destruct s_step.
+    apply (build_system_step sys2 
+        (gstate_morph sys1 sys2 f gstate1) 
+        (gstate_morph sys1 sys2 f gstate2) 
+        sys_chain0 
+        sys_ctx0 
+        (gmsg_morph sys1 sys2 f sys_gmsg0)
+        sys_new_acts0).
+    rewrite <- (sys_coherence sys1 sys2 f).
+    now rewrite sys_recv_some0.
+Defined.
+
+Lemma sm_lift_stm_id {sys} : sm_lift_stm (id_sm sys) = id_stm sys.
+Admitted.
+
+Lemma sm_lift_stm_compose {sys1 sys2 sys3}
+    (g : SystemMorphism sys2 sys3)
+    (f : SystemMorphism sys1 sys2) : 
+    sm_lift_stm (compose_sm g f) = 
+    compose_stm (sm_lift_stm g) (sm_lift_stm f).
+Admitted.
+
+Proposition sys_iso_to_st_iso {sys1 sys2} 
+    (f : SystemMorphism sys1 sys2) (g : SystemMorphism sys2 sys1) : 
+    is_iso_sm f g -> is_iso_stm (sm_lift_stm f) (sm_lift_stm g).
+Proof.
+    intro iso_sm.
+    unfold is_iso_sm, is_iso_stm in *.
+    destruct iso_sm as [iso_sm_l iso_sm_r].
+    split.
+    -   rewrite <- sm_lift_stm_compose.
+        rewrite iso_sm_l.
+        now rewrite sm_lift_stm_id.
+    -   rewrite <- sm_lift_stm_compose.
+        rewrite iso_sm_r.
+        now rewrite sm_lift_stm_id.
+Qed.
 
 
-(* TODO use "accum" somehow? *)
+(* TODO use "accum" somehow? 
 Record SystemTraceMorphism' (sys1 sys2 : ContractSystem) := 
     build_st_morph' {
         (* state morphs, parameterized by states *)
         st_gstate_morph' : GeneralizedState -> GeneralizedState ;
-        sysstep_morph' : forall gstate1 gstate2,
+        sys_step_morph' : forall gstate1 gstate2,
             SystemStep sys1 gstate1 gstate2 -> 
             SystemStep sys2 (st_gstate_morph' gstate1) (st_gstate_morph' gstate2) ;
         sys_state_sync : forall (gstate1 gstate2 : GeneralizedState),
             sys_accum gstate1 = sys_accum gstate2 ->
             sys_accum (st_gstate_morph' gstate1) = sys_accum (st_gstate_morph' gstate2) ;
     }.
-
+*)
 
 End Bisimulation.
 
@@ -231,56 +581,12 @@ End ContractSystemEquivalence.
 (** Operations on Systems of Contracts *)
 Section SystemOperations.
 
-(** Two contract systems can be merged *)
-Section SystemMerge.
-Definition system_merge_inner 
-    (sys1 sys2 : ContractSystem) (name : inner_names sys1) : ContractSystem := 
-    inner_merge sys1 sys2 name.
-
-(* {outer_merge : forall {T} (sys1 : constr T), constr T -> outer_names sys1 -> constr T} *)
-Definition system_merge_outer 
-    (sys1 sys2 : ContractSystem) (name : outer_names sys1) : ContractSystem := 
-    outer_merge sys1 sys2 name.
-
-End SystemMerge.
-
+(* Merges already taken care of *)
 
 (** System quotient *)
 Section SystemQuotient.
 
-(* the system's graph *)
-Definition call_to call : option Address := 
-    match call with 
-    | act_transfer _ _ => None 
-    | act_call addr _ _ => Some addr 
-    | act_deploy _ _ _ => None 
-    end.
 
-(* The type of edges *)
-Record Edges (G1 G2 : GeneralizedContract) : Type := {
-    e_chain : Chain ; 
-    e_ctx : ContractCallContext ; 
-    e_prvstate : SerializedValue ; (* prev state *)
-    e_msg : option SerializedValue ; (* msg *)
-    e_newstate : SerializedValue ; (* new state *)
-    e_nacts : list ActionBody ;
-    linking_act : ActionBody ; (* the action that links the two contracts *)
-    (* there is some transaction for which G1 calls G2 *)
-    e_recv_some : 
-        (* this is a successful call *)
-        wc_receive (wc G1) e_chain e_ctx e_prvstate e_msg = Ok (e_newstate, e_nacts) /\
-        (* which emits the transaction linking_act, *)
-        List.In linking_act e_nacts /\ 
-        (* and it is a call to G2 *)
-        call_to linking_act = Some (addr G2) ;
-}.
-
-(* edges can be composed if they are sequential transactions *)
-Definition edges_compose G1 G2 G3 (e1 : Edges G1 G2) (e2 : Edges G2 G3) := 
-    match linking_act G1 G2 e1 with 
-    | act_call _ _ msg => e_msg G2 G3 e2 = Some msg
-    | _ => False
-    end.
 
 (** Equivalence modulo edges ..? *)
 (* quotient over a path ... ? *)
@@ -296,11 +602,32 @@ End SystemOperations.
 (** An API to go from (strong) contracts to a contract system *)
 Section ContractToSystem.
 
+(* singleton system *)
 
+(* (strong) contract => singleton system *)
+Definition singleton_sys_init bstate caddr : ContractSystem := 
+    match env_contracts bstate caddr with 
+    | Some wc => singleton_ntree {| gc_addr := caddr ; gc_wc := wc ; |} 
+    | None => empty_ntree
+    end.
+
+Definition build_sys bstate sys caddr name : ContractSystem := 
+    match env_contracts bstate caddr with
+    | Some wc => add_tree_at_leaf sys (singleton_ntree {| gc_addr := caddr ; gc_wc := wc ; |}) name
+    | None => sys 
+    end.
+
+(* from a sys_constr of addresses *)
+Definition sys_init bstate (sys_caddrs : ntree Address) : ntree (option GeneralizedContract) := 
+    ntree_funct
+    (fun caddr => 
+        match env_contracts bstate caddr with 
+        | Some wc => Some {| gc_addr := caddr ; gc_wc := wc ; |}
+        | None => None
+        end)
+    sys_caddrs.
 
 End ContractToSystem.
-
-
 
 
 (** Morphisms *)
